pulse/lib/pulse_core/PulseCore.InstantiatedSemantics.fst
@@ -1,6 +1,8 @@
 module PulseCore.InstantiatedSemantics
 module Sem = PulseCore.Semantics2
 module Mem = PulseCore.Memory
+module U = FStar.Universe
+module F = FStar.FunctionalExtensionality
 open Mem
 
 let laws ()
@@ -38,6 +40,7 @@ let laws ()
   ()
 
 let state0 (e:inames) : Sem.state = {
+    max_act = U.raise_t u#0 u#100 unit;
     s = mem;
     is_full_mem = full_mem_pred;
     pred = slprop;
@@ -51,18 +54,74 @@ let state0 (e:inames) : Sem.state = {
 
 let state : Sem.state = state0 Set.empty
 
+let slprop = slprop
+let _eq : squash (slprop == state.pred) = ()
+let emp = emp
+let pure p = pure p
+let ( ** ) p q = p `star` q
+let ( exists* ) #a p = h_exists (F.on_dom a p)
+
+let prop_squash_idem (p:prop)
+  : Tot (squash (p == squash p))
+  = FStar.PropositionalExtensionality.apply p (squash p)
+
+let slprop_equiv p q = Mem.equiv p q
+
+let unsquash (p:squash (slprop_equiv 'p 'q)) : slprop_equiv 'p 'q =
+    prop_squash_idem (slprop_equiv 'p 'q);
+    coerce_eq () p
+    
+let slprop_equiv_refl p = unsquash ()
+    
+let slprop_equiv_elim p q =
+    introduce (p `slprop_equiv` q) ==> p==q
+    with _ . Mem.slprop_extensionality p q
+
+let slprop_equiv_unit p = unsquash ()
+let slprop_equiv_comm p1 p2 = unsquash ()
+let slprop_equiv_assoc p1 p2 p3 = unsquash ()
+module T = FStar.Tactics.V2
+let slprop_equiv_exists 
+    (#a:Type)
+    (p q: a -> slprop)
+    (_:squash (forall x. slprop_equiv (p x) (q x)))
+= introduce forall x. p x == q x
+  with slprop_equiv_elim (p x) (q x);
+  F.extensionality _ _ p q;
+  let pf : squash (eq2 #(F.arrow a (fun _ -> slprop))
+                        (F.on_dom a p)
+                        (F.on_dom a q)) = ()
+  in
+  let x : squash (op_exists_Star p == op_exists_Star q) = _ by (
+      T.norm [delta_only [`%op_exists_Star; `%F.on_dom]; unascribe];
+      let bindings = T.cur_vars() in
+      let bindings = List.Tot.rev bindings in
+      match bindings with
+      | hd::_ -> (
+        match T.term_as_formula hd.sort with
+        | T.Comp (T.Eq _) lhs rhs ->
+          T.grewrite lhs rhs;
+          T.trefl();
+          T.exact (T.binding_to_term hd)
+        | _ -> T.fail "Unexpected type of hd"
+      )
+      | _ ->
+        T.fail "empty bindings"
+  ) in
+  unsquash x
+
 (* The type of general-purpose computations *)
 let stt (a:Type u#a) 
         (pre:slprop)
         (post:a -> slprop)
 : Type0
-= unit -> Dv (Sem.m u#2 u#a #state a pre post)
+= unit -> Dv (Sem.m u#2 u#100 u#a #state a pre post)
 
 let return (#a:Type u#a) (x:a) (p:a -> slprop)
 : stt a (p x) p
 = fun _ -> Sem.ret x p
 
-let bind_stt
+let bind
     (#a:Type u#a) (#b:Type u#b)
     (#pre1:slprop) (#post1:a -> slprop) (#post2:b -> slprop)
     (e1:stt a pre1 post1)
@@ -70,7 +129,7 @@ let bind_stt
 : stt b pre1 post2
 = fun _ -> Sem.mbind (e1()) (fun x -> e2 x ())
 
-let frame_stt
+let frame
   (#a:Type u#a)
   (#pre:slprop) (#post:a -> slprop)
   (frame:slprop)
@@ -78,91 +137,3 @@ let frame_stt
 : stt a (pre `star` frame) (fun x -> post x `star` frame)
 = fun _ -> Sem.frame frame (e())
 
-(* The type of atomic actions *)
-module M = Pulse.MonotonicStateMonad
-let action
-    (a:Type u#a)
-    (except:inames)
-    (pre:slprop)
-    (post:a -> slprop)
-: Type u#(max a 2)
-= frame:slprop ->
-  Sem.mst_sep_aux u#2 u#a state
-    (inames_ok except)
-    (state0 except).invariant
-    a 
-    (pre `star` frame)
-    (fun x -> post x `star` frame)
-
-let return_action
-    (#a:Type u#a)
-    (#except:inames)
-    (#post:a -> slprop)
-    (x:a)
-: action a except (post x) post
-= fun frame -> M.weaken (M.return x)
-
-let bind_action
-     (#a:Type u#a)
-     (#b:Type u#b)
-     (#except:inames)
-     (#pre1 #post1 #post2:_)
-     (f:action a except pre1 post1)
-     (g:(x:a -> action b except (post1 x) post2))
-: action b except pre1 post2
-= fun frame -> M.weaken (M.bind (f frame) (fun x -> g x frame))
-
-let frame_action
-     (#a:Type u#a)
-     (#except:inames)
-     (#pre #post #frame:_)
-     (f:action a except pre post)
-: action a except (pre `star` frame) (fun x -> post x `star` frame)
-= fun frame' -> f (frame `star` frame')
-
-let stt_of_action (#a:Type u#2) #pre #post (m:action a Set.empty pre post)
-: stt a pre post
-= let step (frame:slprop)
-    : Sem.mst_sep state a (pre `star` frame) (fun x -> post x `star` frame)
-    = M.weaken (m frame)
-  in
-  let action : Sem.action state a = {pre=pre; post=post; step} in
-  let m : Sem.m a pre post = Sem.act action in
-  fun _ -> m
-
-module MST = Pulse.MonotonicStateMonad
-
-let mem_action_as_action
-        (a:Type u#a)
-        (except:inames)
-        (req:slprop)
-        (ens: a -> slprop)
-        (act:Mem.action_except a except req ens)
-: action a except req ens
-= fun frame ->
-    let thunk
-      : unit -> MstTot a except req ens frame
-      = fun _ -> act frame
-    in
-    MST.of_msttotal _ _ _ _ thunk
-
-let action_as_mem_action
-        (a:Type u#a)
-        (except:inames)
-        (pre:slprop)
-        (post: a -> slprop) 
-        (act:action a except pre post)
-: Mem.action_except a except pre post
-= fun frame ->
-    let m
-      : MST.mst state.evolves
-                a 
-                (fun s0 -> 
-                    inames_ok except s0 /\
-                    interp ((pre `star` locks_invariant except s0) `star` frame) s0)
-                (fun s0 x s1 ->
-                    inames_ok except s1 /\
-                    interp ((post x `star` locks_invariant except s1) `star` frame) s1)
-      = MST.weaken (act frame)
-    in
-    MST.to_msttotal _ _ _ _ m
