pulse/lib/pulse_core/PulseCore.Memory.fst
@@ -1506,6 +1506,9 @@ let relate_frame_monotonic_2 #a p
 let witness_h_exists #opened_invariants #a p =
   lift_tot_action_with_frame (lift_heap_action_with_frame opened_invariants (H.witness_h_exists p))
 
+let intro_exists #opened_invariants #a p x = 
+  lift_tot_action_with_frame (lift_heap_action_with_frame opened_invariants (H.intro_exists p x))
+
 let lift_h_exists #opened_invariants p = lift_tot_action (lift_heap_action opened_invariants (H.lift_h_exists p))
 
 let elim_pure #opened_invariants p = lift_tot_action (lift_heap_action opened_invariants (H.elim_pure p))
