pulse/lib/pulse_core/PulseCore.InstantiatedSemantics.fsti
@@ -1,0 +1,52 @@
+module PulseCore.InstantiatedSemantics
+
+[@@erasable]
+val slprop : Type u#2
+val emp : slprop
+val pure (p:prop) : slprop
+val ( ** ) (p q : slprop) : slprop
+val ( exists* ) (#a:Type u#a) (p: a -> slprop) : slprop
+val slprop_equiv (p q:slprop) : prop
+
+val slprop_equiv_refl (p:slprop)
+: slprop_equiv p p
+
+val slprop_equiv_elim (p q:slprop)
+: Lemma (p `slprop_equiv` q <==> p==q)
+
+val slprop_equiv_unit (x:slprop)
+: slprop_equiv (emp ** x) x
+
+val slprop_equiv_comm (p1 p2:slprop)
+: slprop_equiv (p1 ** p2) (p2 ** p1)
+
+val slprop_equiv_assoc (p1 p2 p3:slprop)
+: slprop_equiv (p1 ** p2 ** p3) (p1 ** (p2 ** p3))
+
+val slprop_equiv_exists 
+    (#a:Type)
+    (p q: a -> slprop)
+    (_:squash (forall x. slprop_equiv (p x) (q x)))
+: slprop_equiv (op_exists_Star p) (op_exists_Star q)
+
+val stt (a:Type u#a) 
+        (pre:slprop)
+        (post:a -> slprop)
+: Type0
+
+val return (#a:Type u#a) (x:a) (p:a -> slprop)
+: stt a (p x) p
+
+val bind
+    (#a:Type u#a) (#b:Type u#b)
+    (#pre1:slprop) (#post1:a -> slprop) (#post2:b -> slprop)
+    (e1:stt a pre1 post1)
+    (e2:(x:a -> stt b (post1 x) post2))
+: stt b pre1 post2
+
+val frame
+  (#a:Type u#a)
+  (#pre:slprop) (#post:a -> slprop)
+  (frame:slprop)
+  (e:stt a pre post)
+: stt a (pre ** frame) (fun x -> post x ** frame)
